theories/coneris/examples/hash/con_hash_interface2.v
@@ -33,7 +33,7 @@ Class con_hash2 `{!conerisGS Σ} (val_size:nat):= Con_Hash2
   hash_set_gname':Type;
   
   (** * Predicates *)
-  con_hash_inv2 (N:namespace) (f l hm: val) (P:gmap nat nat -> gmap val (list nat) -> iProp Σ) {HP: ∀ m m', Timeless (P m m')} (γ1:hash_view_gname) (γ2: hash_set_gname) (γ3:hash_tape_gname) (γ4:hash_view_gname') (γ5:hash_set_gname') (γ_lock:hash_lock_gname): iProp Σ;
+  con_hash_inv2 (N:namespace) (f l hm: val) (P:gmap nat nat -> gmap val (list nat) -> iProp Σ) {HP: ∀ m m', Timeless (P m m')}  (R:gmap nat nat -> iProp Σ) {HR: ∀ m, Timeless (R m )} (γ1:hash_view_gname) (γ2: hash_set_gname) (γ3:hash_tape_gname) (γ4:hash_view_gname') (γ5:hash_set_gname') (γ_lock:hash_lock_gname): iProp Σ;
   (* concrete_seq_hash {L:seq_hashG Σ} (f:val) (m:gmap nat nat) : iProp Σ;  *)
   hash_tape2 (α:val) (ns:list nat) (γ2: hash_set_gname) (γ3:hash_tape_gname): iProp Σ; 
   hash_tape_auth2 (m:gmap val (list nat)) (γ2 :hash_set_gname) (γ3:hash_tape_gname): iProp Σ;
@@ -57,8 +57,8 @@ Class con_hash2 `{!conerisGS Σ} (val_size:nat):= Con_Hash2
     Timeless (hash_set2 s γ2 γ5); 
   #[global] hash_set_frag_timeless s γ2 γ5 ::
     Timeless (hash_set_frag2 s γ2 γ5); 
-  #[global] con_hash_inv_persistent N f l hm γ1 γ2 γ3 P {HP: ∀ m m', Timeless (P m m')} γ4 γ5 γ_lock ::
-    Persistent (con_hash_inv2 N f l hm P γ1 γ2 γ3 γ4 γ5 γ_lock); 
+  #[global] con_hash_inv_persistent N f l hm γ1 γ2 γ3 P {HP: ∀ m m', Timeless (P m m')} R {HR: ∀ m, Timeless (R m )}γ4 γ5 γ_lock ::
+    Persistent (con_hash_inv2 N f l hm P R γ1 γ2 γ3 γ4 γ5 γ_lock); 
   #[global] hash_frag_persistent v res γ γ2 γ4 ::
     Persistent (hash_frag2 v res γ γ2 γ4);
   (* #[global] hash_set_frag_persistent s γ2 :: *)
@@ -98,10 +98,10 @@ Class con_hash2 `{!conerisGS Σ} (val_size:nat):= Con_Hash2
       hash_tape2 α ns γ2 γ3 -∗ hash_tape2 α ns' γ2 γ3  -∗ False; 
 
   
-  hash_tape_presample N f l hm P {HP: ∀ m m', Timeless (P m m')} m γ_hv γ_set γ_hv' γ γ_set' γ_lock α ns s (ε εO:nonnegreal) E:
+  hash_tape_presample N f l hm P {HP: ∀ m m', Timeless (P m m')} R {HR: ∀ m, Timeless (R m )} m γ_hv γ_set γ_hv' γ γ_set' γ_lock α ns s (ε εO:nonnegreal) E:
   ↑(N.@"rand")⊆E ->
   (INR s + εO * (val_size + 1 - INR s) <= ε * (val_size + 1))%R ->
-  con_hash_inv2 N f l hm P γ_hv γ_set γ γ_hv' γ_set' γ_lock -∗
+  con_hash_inv2 N f l hm P R γ_hv γ_set γ γ_hv' γ_set' γ_lock -∗
     hash_tape_auth2 m γ_set γ -∗ hash_tape2 α ns γ_set γ-∗ ↯ ε -∗
     hash_set2 s γ_set γ_set'-∗
     state_update E E (∃ (n:fin(S val_size)), 
@@ -111,10 +111,10 @@ Class con_hash2 `{!conerisGS Σ} (val_size:nat):= Con_Hash2
           hash_tape2 α (ns++[fin_to_nat n]) γ_set γ ∗ hash_set_frag2 (fin_to_nat n) γ_set γ_set'
       );
 
-  con_hash_presample2  N f l hm P {HP: ∀ m m', Timeless (P m m')} γ_hv γ_set γ_tape γ_hv' γ_set' γ_lock Q
+  con_hash_presample2  N f l hm P {HP: ∀ m m', Timeless (P m m')} R {HR: ∀ m, Timeless (R m )} γ_hv γ_set γ_tape γ_hv' γ_set' γ_lock Q
     E  :
     ↑(N.@"hash") ⊆ E ->
-    con_hash_inv2 N f l hm P γ_hv γ_set γ_tape γ_hv' γ_set' γ_lock -∗
+    con_hash_inv2 N f l hm P R γ_hv γ_set γ_tape γ_hv' γ_set' γ_lock -∗
     (∀ m m', P m m'  -∗
              hash_tape_auth2 m' γ_set γ_tape -∗
              state_update (E∖↑(N.@"hash")) (E∖↑(N.@"hash"))
@@ -124,38 +124,38 @@ Class con_hash2 `{!conerisGS Σ} (val_size:nat):= Con_Hash2
         ∃ m m' m'', Q m m' m''
       ) ; 
 
-  con_hash_init2 N P {HP: ∀ m m', Timeless (P m m')}:
-    {{{ P ∅ ∅ }}}
+  con_hash_init2 N P {HP: ∀ m m', Timeless (P m m')} R {HR: ∀ m, Timeless (R m )}:
+    {{{ P ∅ ∅ ∗ R ∅}}}
       init_hash2 #()
-      {{{ (f:val), RET f; ∃ l hm γ1 γ2 γ3 γ4 γ5 γ_lock, con_hash_inv2 N f l hm P γ1 γ2 γ3 γ4 γ5 γ_lock ∗
+      {{{ (f:val), RET f; ∃ l hm γ1 γ2 γ3 γ4 γ5 γ_lock, con_hash_inv2 N f l hm P R γ1 γ2 γ3 γ4 γ5 γ_lock ∗
                                                   hash_set2 0%nat γ2 γ5
       }}}; 
 
-  con_hash_alloc_tape2 N f l hm P {HP: ∀ m m', Timeless (P m m')} γ1 γ2 γ3 γ4 γ5 γ_lock Q:
-  {{{ con_hash_inv2 N f l hm P γ1 γ2 γ3 γ4 γ5 γ_lock ∗
+  con_hash_alloc_tape2 N f l hm P {HP: ∀ m m', Timeless (P m m')} R {HR: ∀ m, Timeless (R m )} γ1 γ2 γ3 γ4 γ5 γ_lock Q:
+  {{{ con_hash_inv2 N f l hm P R γ1 γ2 γ3 γ4 γ5 γ_lock ∗
       (∀ m m' α, P m m' -∗ ⌜α∉dom m'⌝ -∗ |={⊤∖↑N}=> P m (<[α:=[]]>m') ∗ Q α)
   }}}
       allocate_tape2 #()
       {{{ (α: val), RET α; hash_tape2 α [] γ2 γ3 ∗ Q α }}};  
 
-  con_hash_spec2 N f l hm P {HP: ∀ m m', Timeless (P m m')} γ1 γ2 γ3 γ4 γ5 γ_lock Q1 Q2 α ns (v:nat):
-  {{{ con_hash_inv2 N f l hm P γ1 γ2 γ3 γ4 γ5 γ_lock ∗ hash_tape2 α (ns) γ2 γ3∗
-      ( ∀ m m', P m m' -∗
-                hash_auth2 m γ1 γ2 γ4 γ5-∗
-                ⌜m'!!α=Some ns⌝ -∗
-                |={⊤∖↑N}=>
+  con_hash_spec2  N f l hm P {HP: ∀ m m', Timeless (P m m')} R {HR: ∀ m, Timeless (R m )} γ1 γ2 γ3 γ4 γ5 γ_lock Q1 Q2 α (v:nat):
+  {{{ con_hash_inv2 N f l hm P R γ1 γ2 γ3 γ4 γ5 γ_lock ∗ 
+      ( ∀ m m', R m -∗ P m m' -∗ hash_auth2 m γ1 γ2 γ4 γ5-∗ state_update (⊤∖↑N) (⊤∖↑N)
              match m!!v with
-             | Some res => P m m' ∗ hash_auth2 m γ1 γ2 γ4 γ5 ∗ Q1 res
-             | None => ∃ n ns', ⌜n::ns'=ns⌝ ∗ P (<[v:=n]> m) (<[α:=ns']> m')∗ hash_auth2 (<[v:=n]> m) γ1 γ2 γ4 γ5 ∗
-                                 Q2
+             | Some res => R m ∗ P m m' ∗ hash_auth2 m γ1 γ2 γ4 γ5∗ Q1 res
+             | None => ∃ n ns, hash_tape2 α (n::ns) γ2 γ3 ∗ P m m' ∗
+                              (∀ m'', P m m'' -∗  ⌜m''!!α=Some (n::ns)⌝
+                                      ={⊤∖↑N}=∗ R (<[v:=n]> m) ∗ P (<[v:=n]> m) (<[α:=ns]> m'') ∗
+                                      hash_auth2 (<[v:=n]> m) γ1 γ2 γ4 γ5∗ Q2 n ns)
              end                                        
       )
   }}}
       f #v α
-      {{{ (res:nat), RET (#res);  (hash_tape2 α (ns) γ2 γ3 ∗ Q1 res ∨
-                                 ∃ n ns', ⌜n::ns'=ns⌝ ∗ hash_tape2 α ns' γ2 γ3 ∗ ⌜res=n⌝ ∗ Q2 
+      {{{ (res:nat), RET (#res);  (Q1 res ∨
+                                 ∃ n ns, hash_tape2 α ns γ2 γ3 ∗ ⌜res=n⌝ ∗ Q2 n ns
                                 )
-      }}};
+      }}}
+;
 }.
 
 
@@ -167,7 +167,7 @@ Section test.
   Lemma con_hash_presample_test N f l hm γ1 γ2 γ3 γ4 γ5 γlock  E (ε εI εO:nonnegreal) ns α s :
     ↑N⊆E ->
     (INR s+ εO * (val_size + 1 - INR s) <= ε * (val_size + 1))%R ->
-    con_hash_inv2 N f l hm (λ _ _, True) γ1 γ2 γ3 γ4 γ5 γlock -∗
+    con_hash_inv2 N f l hm (λ _ _, True) (λ _, True) γ1 γ2 γ3 γ4 γ5 γlock -∗
     hash_tape2' α ns γ2 γ3 γ5-∗
     ↯ ε -∗
     hash_set2 s γ2 γ5-∗
@@ -178,7 +178,7 @@ Section test.
       ).
   Proof.
     iIntros (Hsubset Hineq) "#Hinv [Ht Hfrag] Herr Hs".
-    iMod (con_hash_presample2 _ _ _ _ _ _ _ _ _ _ _
+    iMod (con_hash_presample2 _ _ _ _ _ _ _ _ _ _ _ _
             (λ m m' m'', (∃ n : fin (S val_size), hash_tape2 α (ns ++ [fin_to_nat n]) γ2 γ3 ∗
                                                   ( hash_set2 (s +1)%nat γ2 γ5 ∗ ↯ εO) ∗ hash_set_frag2 (fin_to_nat n) _ _))%I with "[//][-Hfrag]") as "Hcont".
     - by apply nclose_subseteq'.
@@ -193,7 +193,7 @@ Section test.
   
     
   Lemma con_hash_spec_test2 N f l hm γ1 γ2 γ3 γ4 γ5 γlock α n ns (v:nat):
-    {{{ con_hash_inv2 N f l hm (λ _ _, True) γ1 γ2 γ3 γ4 γ5 γlock ∗ hash_tape2' α (n::ns) γ2 γ3 γ5 }}}
+    {{{ con_hash_inv2 N f l hm (λ _ _, True) (λ _, True) γ1 γ2 γ3 γ4 γ5 γlock ∗ hash_tape2' α (n::ns) γ2 γ3 γ5 }}}
       f #v α
       {{{ (res:nat), RET (#res);  hash_frag2 v res γ1 γ2 γ4 ∗
                                 (hash_tape2' α ns γ2 γ3 γ5 ∗ ⌜res=n⌝ ∨
@@ -202,38 +202,37 @@ Section test.
       }}}.
   Proof.
     iIntros (Φ) "[#Hinv [Ht Hlis]] HΦ".
-    iApply (con_hash_spec2 _ _ _ _ _ _ _ _ _ _ _ (λ res, hash_frag2 v res γ1 γ2 γ4 ∗ [∗ list] n0 ∈ (n :: ns), hash_set_frag2 n0 γ2 γ5)%I (hash_frag2 v n γ1 γ2 γ4 ∗ [∗ list] n0 ∈ (ns), hash_set_frag2 n0 γ2 γ5) with "[$Hinv $Ht Hlis]").
-    - iIntros (??) "_ Hauth %".
+    iApply (con_hash_spec2 _ _ _ _ _ _ _ _ _ _ _ _ (λ res, hash_tape2 _ _ _ _ ∗ hash_frag2 v res γ1 γ2 γ4 ∗ [∗ list] n0 ∈ (n :: ns), hash_set_frag2 n0 γ2 γ5)%I (λ n' ns', ⌜n=n'⌝ ∗ ⌜ns=ns'⌝ ∗ hash_frag2 v n γ1 γ2 γ4 ∗ [∗ list] n0 ∈ (ns), hash_set_frag2 n0 γ2 γ5)%I with "[$Hinv Ht Hlis]").
+    - iIntros (??) "_ _ Hauth".
       case_match.
       + iDestruct (hash_auth_duplicate with "[$]") as "#$"; first done. by iFrame.
       + iDestruct "Hlis" as "[H1 Hlis]".
         iMod (hash_auth_insert with "[$][$]") as "H"; first done.
         iDestruct (hash_auth_duplicate with "[$]") as "#$"; first by rewrite lookup_insert.
-        iFrame. iModIntro. iExists _. done.
-    - iNext. iIntros (res) "[(?&?&?)|(%&%&%&?&%&H&?)]".
+        iFrame. iModIntro. iIntros. iPureIntro. done. 
+    - iNext. iIntros (res) "[(?&?&?)|(%&%&?&->&->&->&?&?)]".
       + iApply "HΦ". iFrame. iRight. iFrame.
-      + iApply "HΦ". simplify_eq. iFrame "H". iLeft. by iFrame.
+      + iApply "HΦ". simplify_eq. iFrame. iLeft. by iFrame. 
   Qed.
 
   Lemma con_hash_spec_hashed_before2 N f l hm γ1 γ2 γ3 γ4 γ5 γlock α ns res (v:nat):
-    {{{ con_hash_inv2 N f l hm (λ _ _, True) γ1 γ2 γ3 γ4 γ5 γlock ∗ hash_tape2' α ns γ2 γ3 γ5 ∗ hash_frag2 v res γ1 γ2 γ4}}}
+    {{{ con_hash_inv2 N f l hm (λ _ _, True) (λ _, True) γ1 γ2 γ3 γ4 γ5 γlock ∗ hash_tape2' α ns γ2 γ3 γ5 ∗ hash_frag2 v res γ1 γ2 γ4}}}
       f #v α
       {{{ RET (#res);  hash_frag2 v res γ1 γ2 γ4 ∗
                        (hash_tape2' α ns γ2 γ3 γ5)
       }}}.
   Proof. 
     iIntros (Φ) "(#Hinv & [Ht ?] & #Hf) HΦ".
-    iApply (con_hash_spec2 _ _ _ _ _ _ _ _ _ _ _(λ res' , ⌜res=res'⌝ ∗ hash_frag2 v res γ1 γ2 γ4  )%I (False) with "[$Hinv $Ht]").
-    - iIntros (??) "_ Hauth %".
+    iApply (con_hash_spec2 _ _ _ _ _ _ _ _ _ _ _ _ (λ res' , ⌜res=res'⌝ ∗ hash_frag2 v res γ1 γ2 γ4 ∗ hash_tape2 _ _ _ _ )%I (λ _ _, ⌜False⌝)%I with "[$Hinv Ht]").
+    - iIntros (??) "_ _ Hauth".
       case_match.
       + iDestruct (hash_auth_frag_agree with "[$][$]") as "%".
         simplify_eq. iDestruct (hash_auth_duplicate with "[$]") as "#$"; first done.
         iFrame. by done. 
       + iDestruct (hash_auth_frag_agree with "[$][$]") as "%".
         simplify_eq.
-    - iNext. iIntros (res') "[[?[->?]]|(%&%&%&?&?&%)]".
-      + iApply "HΦ". iFrame.
-      + done.
+    - iNext. iIntros (res') "[[->[??]]|(%&%&?&%&[])]".
+      iApply "HΦ". iFrame.
   Qed.
   
 End test.
