theories/coneris/examples/hash/con_hash_interface3.v
@@ -41,7 +41,7 @@ Class con_hash3 `{!conerisGS Σ} (val_size:nat) (max_hash_size:nat) (Hpos:0<max_
   hash_token_gname:Type;
   
   (** * Predicates *)
-  con_hash_inv3 (N:namespace) (f l hm: val) (P:gmap nat nat -> gmap val (list nat) -> iProp Σ) {HP: ∀ m m', Timeless (P m m')} (γ1:hash_view_gname) (γ2: hash_set_gname) (γ3:hash_tape_gname) (γ4:hash_view_gname') (γ5:hash_set_gname') (γ6: hash_token_gname) (γ_lock:hash_lock_gname): iProp Σ;
+  con_hash_inv3 (N:namespace) (f l hm: val) (P:gmap nat nat -> gmap val (list nat) -> iProp Σ) {HP: ∀ m m', Timeless (P m m')}  (R:gmap nat nat -> iProp Σ) {HR: ∀ m, Timeless (R m )} (γ1:hash_view_gname) (γ2: hash_set_gname) (γ3:hash_tape_gname) (γ4:hash_view_gname') (γ5:hash_set_gname') (γ6: hash_token_gname) (γ_lock:hash_lock_gname): iProp Σ;
   (* concrete_seq_hash {L:seq_hashG Σ} (f:val) (m:gmap nat nat) : iProp Σ;  *)
   hash_tape3 (α:val) (ns:list nat) (γ2: hash_set_gname) (γ3:hash_tape_gname): iProp Σ; 
   hash_tape_auth3 (m:gmap val (list nat)) (γ2 :hash_set_gname) (γ3:hash_tape_gname): iProp Σ;
@@ -68,8 +68,8 @@ Class con_hash3 `{!conerisGS Σ} (val_size:nat) (max_hash_size:nat) (Hpos:0<max_
     Timeless (hash_set_frag3 s γ2 γ5); 
   #[global] hash_token_timeless s γ6 ::
     Timeless (hash_token3 s γ6); 
-  #[global] con_hash_inv_persistent N f l hm γ1 γ2 γ3 P {HP: ∀ m m', Timeless (P m m')} γ4 γ5 γ6 γ_lock ::
-    Persistent (con_hash_inv3 N f l hm P γ1 γ2 γ3 γ4 γ5 γ6 γ_lock); 
+  #[global] con_hash_inv_persistent N f l hm γ1 γ2 γ3 P {HP: ∀ m m', Timeless (P m m')} R {HR: ∀ m, Timeless (R m )} γ4 γ5 γ6 γ_lock ::
+    Persistent (con_hash_inv3 N f l hm P R γ1 γ2 γ3 γ4 γ5 γ6 γ_lock); 
   #[global] hash_frag_persistent v res γ γ2 γ4 ::
     Persistent (hash_frag3 v res γ γ2 γ4);
   (* #[global] hash_set_frag_persistent s γ2 :: *)
@@ -111,9 +111,9 @@ Class con_hash3 `{!conerisGS Σ} (val_size:nat) (max_hash_size:nat) (Hpos:0<max_
   hash_token3 (n+n') γ6 ⊣⊢hash_token3 n γ6 ∗ hash_token3 n' γ6;
 
   
-  hash_tape_presample N f l hm P {HP: ∀ m m', Timeless (P m m')} m γ_hv γ_set γ_hv' γ_token γ γ6 γ_set' γ_lock α ns s E:
+  hash_tape_presample N f l hm P {HP: ∀ m m', Timeless (P m m')} R {HR: ∀ m, Timeless (R m )} m γ_hv γ_set γ_hv' γ_token γ γ6 γ_set' γ_lock α ns s E:
   ↑(N.@"rand")⊆E ->
-  con_hash_inv3 N f l hm P γ_hv γ_set γ γ_hv' γ_set' γ_token γ_lock -∗
+  con_hash_inv3 N f l hm P R γ_hv γ_set γ γ_hv' γ_set' γ_token γ_lock -∗
   hash_tape_auth3 m γ_set γ -∗
   hash_tape3 α ns γ_set γ-∗
   ↯ (amortized_error val_size max_hash_size Hpos) -∗
@@ -125,10 +125,10 @@ Class con_hash3 `{!conerisGS Σ} (val_size:nat) (max_hash_size:nat) (Hpos:0<max_
           hash_tape3 α (ns++[fin_to_nat n]) γ_set γ ∗ hash_set_frag3 (fin_to_nat n) γ_set γ_set'
       ); 
 
-  con_hash_presample3  N f l hm P {HP: ∀ m m', Timeless (P m m')} γ_hv γ_set γ_tape γ_hv' γ_set' γ_token γ_lock Q
+  con_hash_presample3  N f l hm P {HP: ∀ m m', Timeless (P m m')} R {HR: ∀ m, Timeless (R m )} γ_hv γ_set γ_tape γ_hv' γ_set' γ_token γ_lock Q
     E  :
     ↑(N) ⊆ E ->
-    con_hash_inv3 N f l hm P γ_hv γ_set γ_tape γ_hv' γ_set' γ_token γ_lock -∗
+    con_hash_inv3 N f l hm P R γ_hv γ_set γ_tape γ_hv' γ_set' γ_token γ_lock -∗
     (∀ m m' s, P m m'  -∗
                hash_set3 s γ_set γ_set' γ_token -∗
              hash_tape_auth3 m' γ_set γ_tape -∗
@@ -139,37 +139,36 @@ Class con_hash3 `{!conerisGS Σ} (val_size:nat) (max_hash_size:nat) (Hpos:0<max_
         ∃ m m' m'' s , Q m m' m'' s
       ) ; 
 
-  con_hash_init3 N P {HP: ∀ m m', Timeless (P m m')}:
-    {{{ P ∅ ∅ }}}
+  con_hash_init3 N P {HP: ∀ m m', Timeless (P m m')}R {HR: ∀ m, Timeless (R m )} :
+    {{{ P ∅ ∅ ∗ R ∅}}}
       init_hash3 #()
-      {{{ (f:val), RET f; ∃ l hm γ1 γ2 γ3 γ4 γ5 γ_token γ_lock, con_hash_inv3 N f l hm P γ1 γ2 γ3 γ4 γ5 γ_token γ_lock ∗  hash_token3 max_hash_size γ_token
+      {{{ (f:val), RET f; ∃ l hm γ1 γ2 γ3 γ4 γ5 γ_token γ_lock, con_hash_inv3 N f l hm P R γ1 γ2 γ3 γ4 γ5 γ_token γ_lock ∗  hash_token3 max_hash_size γ_token
       }}}; 
 
-  con_hash_alloc_tape3 N f l hm P {HP: ∀ m m', Timeless (P m m')} γ1 γ2 γ3 γ4 γ5 γ_token γ_lock Q:
-  {{{ con_hash_inv3 N f l hm P γ1 γ2 γ3 γ4 γ5 γ_token γ_lock ∗
+  con_hash_alloc_tape3 N f l hm P {HP: ∀ m m', Timeless (P m m')} R {HR: ∀ m, Timeless (R m )} γ1 γ2 γ3 γ4 γ5 γ_token γ_lock Q:
+  {{{ con_hash_inv3 N f l hm P R γ1 γ2 γ3 γ4 γ5 γ_token γ_lock ∗
       (∀ m m' α, P m m' -∗ ⌜α∉dom m'⌝ -∗ |={⊤∖↑N}=> P m (<[α:=[]]>m') ∗ Q α)
   }}}
       allocate_tape3 #()
       {{{ (α: val), RET α; hash_tape3 α [] γ2 γ3 ∗ Q α }}};  
 
-  con_hash_spec3 N f l hm P {HP: ∀ m m', Timeless (P m m')} γ1 γ2 γ3 γ4 γ5 γ_token γ_lock Q1 Q2 α ns (v:nat):
-  {{{ con_hash_inv3 N f l hm P γ1 γ2 γ3 γ4 γ5 γ_token γ_lock ∗ hash_tape3 α (ns) γ2 γ3∗
-      ( ∀ m m', P m m' -∗
-                hash_auth3 m γ1 γ2 γ4 γ5-∗
-                ⌜m'!!α=Some ns⌝ -∗
-                |={⊤∖↑N}=>
+  con_hash_spec3 N f l hm P {HP: ∀ m m', Timeless (P m m')} R {HR: ∀ m, Timeless (R m )} γ1 γ2 γ3 γ4 γ5 γ_token γ_lock Q1 Q2 α (v:nat):
+  {{{ con_hash_inv3 N f l hm P R γ1 γ2 γ3 γ4 γ5 γ_token γ_lock ∗ 
+      ( ∀ m m', R m -∗ P m m' -∗ hash_auth3 m γ1 γ2 γ4 γ5-∗ state_update (⊤∖↑N) (⊤∖↑N)
              match m!!v with
-             | Some res => P m m' ∗ hash_auth3 m γ1 γ2 γ4 γ5 ∗ Q1 res
-             | None => ∃ n ns', ⌜n::ns'=ns⌝ ∗ P (<[v:=n]> m) (<[α:=ns']> m')∗ hash_auth3 (<[v:=n]> m) γ1 γ2 γ4 γ5 ∗
-                                 Q2
+             | Some res => R m ∗ P m m' ∗ hash_auth3 m γ1 γ2 γ4 γ5∗ Q1 res
+             | None => ∃ n ns, hash_tape3 α (n::ns) γ2 γ3 ∗ P m m' ∗
+                              (∀ m'', P m m'' -∗  ⌜m''!!α=Some (n::ns)⌝
+                                      ={⊤∖↑N}=∗ R (<[v:=n]> m) ∗ P (<[v:=n]> m) (<[α:=ns]> m'') ∗
+                                      hash_auth3 (<[v:=n]> m) γ1 γ2 γ4 γ5∗ Q2 n ns)
              end                                        
       )
   }}}
       f #v α
-      {{{ (res:nat), RET (#res);  (hash_tape3 α (ns) γ2 γ3 ∗ Q1 res ∨
-                                 ∃ n ns', ⌜n::ns'=ns⌝ ∗ hash_tape3 α ns' γ2 γ3 ∗ ⌜res=n⌝ ∗ Q2 
+      {{{ (res:nat), RET (#res);  (Q1 res ∨
+                                 ∃ n ns, hash_tape3 α ns γ2 γ3 ∗ ⌜res=n⌝ ∗ Q2 n ns
                                 )
-      }}};
+      }}}
 }.
 
 
@@ -183,7 +182,7 @@ Section test.
 
   Lemma con_hash_presample_test N f l hm γ1 γ2 γ3 γ4 γ5 γlock γ_token E ns α :
     ↑N⊆E ->
-    con_hash_inv3 N f l hm (λ _ _, True) γ1 γ2 γ3 γ4 γ5 γ_token γlock -∗
+    con_hash_inv3 N f l hm (λ _ _, True) (λ _, True )γ1 γ2 γ3 γ4 γ5 γ_token γlock -∗
     hash_tape3' α ns γ2 γ3 γ5-∗
     ↯ (amortized_error val_size max_hash_size max_hash_size_pos) -∗
     hash_token3 1 γ_token -∗
@@ -192,7 +191,7 @@ Section test.
       ).
   Proof.
     iIntros (Hsubset) "#Hinv [Ht Hfrag] Herr Htoken".
-    iMod (con_hash_presample3 _ _ _ _ _ _ _ _ _ _ _ _
+    iMod (con_hash_presample3 _ _ _ _ _ _ _ _ _ _ _ _ _
             (λ m m' m'' _, (∃ n : fin (S val_size), hash_tape3 α (ns ++ [fin_to_nat n]) γ2 γ3 ∗
                                                     hash_set_frag3 (fin_to_nat n) _ _))%I with "[//][-Hfrag]") as "Hcont".
     - done. 
@@ -206,7 +205,7 @@ Section test.
   
     
   Lemma con_hash_spec_test3 N f l hm γ1 γ2 γ3 γ4 γ5 γ_token γlock α n ns (v:nat):
-    {{{ con_hash_inv3 N f l hm (λ _ _, True) γ1 γ2 γ3 γ4 γ5 γ_token  γlock ∗ hash_tape3' α (n::ns) γ2 γ3 γ5 }}}
+    {{{ con_hash_inv3 N f l hm (λ _ _, True) (λ _, True )γ1 γ2 γ3 γ4 γ5 γ_token  γlock ∗ hash_tape3' α (n::ns) γ2 γ3 γ5 }}}
       f #v α
       {{{ (res:nat), RET (#res);  hash_frag3 v res γ1 γ2 γ4 ∗
                                 (hash_tape3' α ns γ2 γ3 γ5 ∗ ⌜res=n⌝ ∨
@@ -215,38 +214,37 @@ Section test.
       }}}.
   Proof.
     iIntros (Φ) "[#Hinv [Ht Hlis]] HΦ".
-    iApply (con_hash_spec3 _ _ _ _ _ _ _ _ _ _ _ _ (λ res, hash_frag3 v res γ1 γ2 γ4 ∗ [∗ list] n0 ∈ (n :: ns), hash_set_frag3 n0 γ2 γ5)%I (hash_frag3 v n γ1 γ2 γ4 ∗ [∗ list] n0 ∈ (ns), hash_set_frag3 n0 γ2 γ5) with "[$Hinv $Ht Hlis]").
-    - iIntros (??) "_ Hauth %".
+    iApply (con_hash_spec3 _ _ _ _ _ _ _ _ _ _ _ _ _ (λ res, hash_frag3 v res γ1 γ2 γ4 ∗ hash_tape3 _ _ _ _ ∗ [∗ list] n0 ∈ (n :: ns), hash_set_frag3 n0 γ2 γ5 )%I (λ n' ns', ⌜n=n'⌝ ∗ ⌜ns = ns'⌝ ∗ hash_frag3 v n γ1 γ2 γ4 ∗ [∗ list] n0 ∈ (ns), hash_set_frag3 n0 γ2 γ5)%I with "[$Hinv Ht Hlis]").
+    - iIntros (??) "_ _ Hauth".
       case_match.
       + iDestruct (hash_auth_duplicate with "[$]") as "#$"; first done. by iFrame.
       + iDestruct "Hlis" as "[H1 Hlis]".
         iMod (hash_auth_insert with "[$][$]") as "H"; first done.
         iDestruct (hash_auth_duplicate with "[$]") as "#$"; first by rewrite lookup_insert.
-        iFrame. iModIntro. iExists _. done.
-    - iNext. iIntros (res) "[(?&?&?)|(%&%&%&?&%&H&?)]".
+        iFrame. iModIntro. iIntros. iPureIntro. done. 
+    - iNext. iIntros (res) "[(?&?&?)|(%&%&?&->&->&->&?&?)]".
       + iApply "HΦ". iFrame. iRight. iFrame.
-      + iApply "HΦ". simplify_eq. iFrame "H". iLeft. by iFrame.
+      + iApply "HΦ". simplify_eq. iFrame. iLeft. by iFrame.
   Qed.
 
   Lemma con_hash_spec_hashed_before3 N f l hm γ1 γ2 γ3 γ4 γ5 γtoken γlock α ns res (v:nat):
-    {{{ con_hash_inv3 N f l hm (λ _ _, True) γ1 γ2 γ3 γ4 γ5 γtoken γlock ∗ hash_tape3' α ns γ2 γ3 γ5 ∗ hash_frag3 v res γ1 γ2 γ4}}}
+    {{{ con_hash_inv3 N f l hm (λ _ _, True) (λ _, True) γ1 γ2 γ3 γ4 γ5 γtoken γlock ∗ hash_tape3' α ns γ2 γ3 γ5 ∗ hash_frag3 v res γ1 γ2 γ4}}}
       f #v α
       {{{ RET (#res);  hash_frag3 v res γ1 γ2 γ4 ∗
                        (hash_tape3' α ns γ2 γ3 γ5)
       }}}.
   Proof. 
     iIntros (Φ) "(#Hinv & [Ht ?] & #Hf) HΦ".
-    iApply (con_hash_spec3 _ _ _ _ _ _ _ _ _ _ _ _(λ res' , ⌜res=res'⌝ ∗ hash_frag3 v res γ1 γ2 γ4  )%I (False) with "[$Hinv $Ht]").
-    - iIntros (??) "_ Hauth %".
+    iApply (con_hash_spec3 _ _ _ _ _ _ _ _ _ _ _ _ _(λ res' , ⌜res=res'⌝ ∗ hash_tape3 _ _ _ _ ∗hash_frag3 v res γ1 γ2 γ4  )%I (λ _ _, ⌜False⌝)%I with "[$Hinv Ht]").
+    - iIntros (??) "_ _ Hauth".
       case_match.
       + iDestruct (hash_auth_frag_agree with "[$][$]") as "%".
         simplify_eq. iDestruct (hash_auth_duplicate with "[$]") as "#$"; first done.
         iFrame. by done. 
       + iDestruct (hash_auth_frag_agree with "[$][$]") as "%".
         simplify_eq.
-    - iNext. iIntros (res') "[[?[->?]]|(%&%&%&?&?&%)]".
-      + iApply "HΦ". iFrame.
-      + done.
+    - iNext. iIntros (res') "[[->[??]]|(%&%&?&?&[])]".
+      iApply "HΦ". iFrame.
   Qed.
   
 End test.
